Weidenbach_Book/CDCL_NOT.thy
@@ -2477,7 +2477,8 @@ locale cdcl\<^sub>N\<^sub>O\<^sub>T_increasing_restarts_ops =
        \<Longrightarrow> \<mu> A U \<le> \<mu>_bound A T" and
     measure_bound4: "\<And>A T U. cdcl\<^sub>N\<^sub>O\<^sub>T_inv T \<Longrightarrow> bound_inv A T \<Longrightarrow> cdcl\<^sub>N\<^sub>O\<^sub>T\<^sup>*\<^sup>* T U
        \<Longrightarrow> \<mu>_bound A U \<le> \<mu>_bound A T" and
-    cdcl\<^sub>N\<^sub>O\<^sub>T_restart_inv: "\<And>A U V. cdcl\<^sub>N\<^sub>O\<^sub>T_inv U \<Longrightarrow> restart U V \<Longrightarrow> bound_inv A U \<Longrightarrow> bound_inv A V" and
+    cdcl\<^sub>N\<^sub>O\<^sub>T_restart_inv: "\<And>A U V. cdcl\<^sub>N\<^sub>O\<^sub>T_inv U \<Longrightarrow> restart U V \<Longrightarrow> bound_inv A U \<Longrightarrow> bound_inv A V"
+      and
     exists_bound: "\<And>R S. cdcl\<^sub>N\<^sub>O\<^sub>T_inv R \<Longrightarrow> restart R S \<Longrightarrow> \<exists>A. bound_inv A S" and
     cdcl\<^sub>N\<^sub>O\<^sub>T_inv: "\<And>S T. cdcl\<^sub>N\<^sub>O\<^sub>T_inv S \<Longrightarrow> cdcl\<^sub>N\<^sub>O\<^sub>T S T \<Longrightarrow> cdcl\<^sub>N\<^sub>O\<^sub>T_inv T" and
     cdcl\<^sub>N\<^sub>O\<^sub>T_inv_restart: "\<And>S T. cdcl\<^sub>N\<^sub>O\<^sub>T_inv S \<Longrightarrow> restart S T \<Longrightarrow> cdcl\<^sub>N\<^sub>O\<^sub>T_inv T"
